src/freeboogie/trunk/FreeBoogie/test/functional/tc.ok/pass_outref.bpl
@@ -3,6 +3,8 @@ procedure swap(x : ref, y : ref) returns (xx : ref, yy : ref);
   ensures y == xx;
 
 implementation swap(x : ref, y : ref) returns (xx : ref, yy : ref) {
+  var xx_1 : ref;
+  var yy_1 : ref;
 entry:
   assume yy_1 == x;
   assume xx_1 == y;
@@ -20,6 +22,8 @@ procedure even(x : int) returns (y : int);
   ensures y % 2 == 0;
 
 implementation even(x : int) returns (y : int) {
+  var y_1 : int;
+  var y_2 : int;
 entry:
   assume y_1 == x;
   goto a, b;
@@ -44,16 +48,22 @@ post_check:
 
 var mem : [ref] int;
 
+procedure store1d<x,z>([x]z,x,z) returns (z);
+procedure store2d<x,y,z>([x,y]z,x,y,z) returns (z);
+
 procedure pswap(x : ref, y : ref);
   ensures mem[x] == old(mem[y]);
   ensures mem[y] == old(mem[x]);
 
 implementation pswap(x : ref, y : ref) {
   var tmp : int;
+  var tmp_1 : int;
+  var mem_1 : [ref]int;
+  var mem_2 : [ref]int;
 entry:
   assume tmp_1 == mem[x];
-  assume mem_1 == store(mem, x, mem[y]); // ** array store **
-  assume mem_2 == store(mem_1, y, tmp);
+  assume mem_1 == store1d(mem, x, mem[y]); // ** array store **
+  assume mem_2 == store1d(mem_1, y, tmp);
   goto post_check;
 
 post_check:
