src/freeboogie/trunk/FreeBoogie/editors/vim/syntax/antlr.vim
@@ -1,0 +1,47 @@
+" Vim syntax file
+" Language:    ANTLR 3
+" Maintainer:  Radu Grigore <radugrigore@gmail.com>
+" Version:     0.0
+" Last Change: 18 Mar 2008
+
+" TODO: How to detect that the file is ANTLR? (pccts has the same extension)
+" TODO: Is it possible to figure out the language in semantic actions?
+
+" Magic incantation from the VIM7 user manual
+if exists("b:current_syntax")
+   finish
+endif
+
+" Assume that the code inside semantic actions is Java
+syn include @javaCode <sfile>:p:h/java.vim
+syn region antlrAction start=/{/ end=/}/ contains=@javaCode,antlrAction,antlrId
+
+" Some keywords
+syn keyword antlrKeywords options tokens parser lexer tree grammar header
+syn keyword antlrKeywords protected public private returns throws exception
+
+" Operators
+syn match antlrOp /|\|\*\|?\|:\|\~/
+syn match antlrId /\$\w\+/
+
+" Inlined tokens
+syn region antlrToken1 start=/'/ end=/'/ skip=/\\'/
+syn region antlrToken2 start=/"/ end=/"/ skip=/\\"/
+
+" Comments
+syn match antlrComment /\/\/.*/
+syn region antlrBlockComment start='/\*' end='\*/'
+
+" The colors
+hi def link antlrToken1       String
+hi def link antlrToken2       String
+hi def link antlrKeywords     Keyword
+hi def link antlrComment      Comment
+hi def link antlrBlockComment Comment
+hi def link antlrOp           Operator
+hi def link antlrId           Identifier
+
+" Magic incantation from section 44.12 in the VIM7 user manual
+let b:current_syntax = "antlr"
+
+" vim:spell:et:sw=3:ts=3:
